Reorganisation of logical relations code

src/Language/PlutusIR/Semantics/SemanticEquivalence/LogicalRelation/RelationalModel.v
@@ -1,63 +1,15 @@
 Require Import PlutusCert.Language.PlutusIR.Semantics.Static.
 Require Import PlutusCert.Language.PlutusIR.Semantics.Dynamic.
-Require Import PlutusCert.Language.PlutusIR.Semantics.TypeSafety.SubstitutionPreservesTyping.
-Require Import PlutusCert.Language.PlutusIR.Semantics.TypeSafety.Preservation.
-Require Import PlutusCert.Util.Map.Mupdate.
+Require Import PlutusCert.Language.PlutusIR.Semantics.SemanticEquivalence.LogicalRelation.Tymapping.
 
 From Coq Require Import Lia.
+
 Require Import Arith.
 Require Import Coq.Lists.List.
 Require Import Coq.Strings.String.
+
+Local Open Scope list_scope.
 Local Open Scope string_scope.
-
-(** ** Type mappings
-
-    We denote a type mapping by rho. A type mapping maps
-    type variables to a triplet of a step-indexed relation and two types.
-*)
-Definition tymapping := list (tyname * ((nat -> Term -> Term -> Prop) * Ty * Ty)).
-
-
-(** Semantic substitution for the type variable a *)
-Fixpoint sem (rho : tymapping) (a : tyname) : option (nat -> Term -> Term -> Prop) :=
-  match rho with
-  | nil => None
-  | (a', (Chi, _ , _)) :: rho' => 
-      if a =? a' then Datatypes.Some Chi else sem rho' a
-  end.
-
-
-(** (Left) syntactic substitution for the type variable a *)
-Fixpoint syn1 (rho : tymapping) (a : tyname) : option Ty :=
-  match rho with
-  | nil => None
-  | (a', (_, T1, _)) :: rho' => 
-      if a =? a' then Datatypes.Some T1 else syn1 rho' a
-  end.
-
-(** (Right) syntactic substitution for the type variable a *)
-Fixpoint syn2 (rho : tymapping) (a : tyname) : option Ty :=
-  match rho with
-  | nil => None
-  | (a', (_, _, T2)) :: rho' => 
-      if a =? a' then Datatypes.Some T2 else syn2 rho' a
-  end.
-
-(** (Left) syntactic substitutions in rho *)
-Fixpoint msyn1 (rho : tymapping) : list (tyname * Ty) :=
-  match rho with
-  | nil => nil
-  | (a', (_, T1, _)) :: rho' => 
-      (a', T1) :: msyn1 rho'
-  end.
-
-(** (Right) syntactic substitutions in rho *)
-Fixpoint msyn2 (rho : tymapping) : list (tyname * Ty) :=
-  match rho with
-  | nil => nil
-  | (a', (_, _, T2)) :: rho' => 
-      (a', T2) :: msyn2 rho'
-  end.
 
 Definition Rel 
     (T T' : Ty) 
@@ -65,18 +17,18 @@ Definition Rel
     : Prop :=
   forall j v v',
     Chi j v v' ->
-    (* value v /\ value v' /\ *)
-    empty ,, empty |-+ v : T /\
-    (empty ,, empty |-+ v' : T') /\ 
+    0 < j ->
+    (exists Tn, normalise T Tn /\ (empty ,, empty |-+ v : Tn)) /\
+    (exists Tn', normalise T' Tn' /\ (empty ,, empty |-+ v' : Tn')) /\ 
     forall i,
       i <= j ->
       Chi i v v'.
 
+(** Relation interpational of types as computations and values.
 
-
-(** ** Relation interpation for computations and values *)
-
-(** RV = Relational interpretation for values, RC = Relation interpretation for computations *)
+    RV = Relational interpretation for values
+    RC = Relation interpretation for computations
+*)
 Equations? RC (k : nat) (T : Ty) (rho : tymapping) (e e' : Term) : Prop by wf k :=
   RC k T rho e e' =>
     (* RC *)
@@ -86,70 +38,66 @@ Equations? RC (k : nat) (T : Ty) (rho : tymapping) (e e' : Term) : Prop by wf k 
       exists e'_f j', e' =[j']=> e'_f /\
       
       (* RV *)
-      (empty ,, empty |-+ e_f : (msubstT (msyn1 rho) T)) /\
-      (empty ,, empty |-+ e'_f : (msubstT (msyn2 rho) T)) /\
-      match T with
+      (exists Tn, normalise (msubstT (msyn1 rho) T) Tn /\ (empty ,, empty |-+ e_f : Tn)) /\
+      (exists Tn', normalise (msubstT (msyn2 rho) T) Tn' /\  (empty ,, empty |-+ e'_f : Tn')) /\
+      
+      ( 
+        ~ is_error e_f /\
+        ~ is_error e'_f /\
+        (
+          match T with
 
-        (* RV for type variable *)
-        | Ty_Var a =>
-            forall Chi,
-            sem rho a = Datatypes.Some Chi ->  
-            Chi (k - j) e_f e'_f
+          (* RV for type variable *)
+          | Ty_Var a =>
+              forall Chi,
+                sem rho a = Datatypes.Some Chi ->  
+                Chi (k - j) e_f e'_f
 
-        (* RV for type lambda *)
-        | Ty_Lam bX K T =>
-            False
+          (* RV for type lambda *)
+          | Ty_Lam bX K T =>
+              False
 
-        (* RV for type application *)
-        | Ty_App T1 T2 => 
-            False
+          (* RV for type application *)
+          | Ty_App T1 T2 => 
+              False
 
-        (* RV for built-in types *)
-        | Ty_Builtin st => 
-            exists sv sv',
+          (* RV for built-in types *)
+          | Ty_Builtin st => 
+              exists sv sv',
+                (* Determine the shape of e_f and e'_f *)
+                e_f = Constant sv /\
+                e'_f = Constant sv' /\
+                (* Syntactic equality *)
+                e_f = e'_f
+
+          (* RV for function types *)
+          | Ty_Fun T1 T2 =>
               (* Determine the shape of e_f and e'_f *)
-              e_f = Constant sv /\
-              e'_f = Constant sv' /\
-              (* Syntactic equality *)
-              e_f = e'_f
-
-        (* RV for function types *)
-        | Ty_Fun T1 T2 =>
-            (
-              (* Determine the shape of e_f and e'_f *)
-              exists x e_body x' e'_body,   
-                LamAbs x (msubstT (msyn1 rho) T1) e_body = e_f /\
-                LamAbs x' (msubstT (msyn2 rho) T1) e'_body = e'_f /\
+              exists x e_body x' e'_body T1p,
+                normalise T1p T1 /\   
+                LamAbs x (msubstT (msyn1 rho) T1p) e_body = e_f /\
+                LamAbs x' (msubstT (msyn2 rho) T1p) e'_body = e'_f /\
                 (* Extensional equivalence *)
                 forall i (Hlt_i : i < k - j) v_0 v'_0,
                   value v_0 /\ value v'_0 /\ RC i T1 rho v_0 v'_0 ->
                   RC i T2 rho <{ [v_0 / x] e_body }> <{ [v'_0 / x'] e'_body }>
-            ) \/ (
-              (* Determine the shape of e_f and e'_f*)
-              exists f args f' args',
-                ExtBuiltin f args = e_f /\
-                ExtBuiltin f' args' = e'_f /\
-                (* Extensional equivalence*)
-                forall i (Hlt_i : i < k - j) v_0 v'_0,
-                  value v_0 /\ value v'_0 /\ RC i T1 rho v_0 v'_0 ->
-                  RC i T2 rho (ExtBuiltin f (v_0 :: args)) (ExtBuiltin f' (v'_0 :: args'))
-            )
 
-        (* RV for recursive types *)
-        | Ty_IFix F T =>
-            exists v_0 v'_0,
-              (* Determine the shape of e_f and e_f' *)
-              e_f = IWrap (msubstT (msyn1 rho) F) (msubstT (msyn1 rho) T) v_0 /\
-              e'_f = IWrap (msubstT (msyn2 rho) F) (msubstT (msyn2 rho) T) v'_0 /\
-              (* Uwrap *)
-              forall i (Hlt_i : i < k - j) K S,
-                empty |-* (msubstT (msyn2 rho) T) : K ->
-                normalise (unwrapIFix F K T) S ->
-                RC i S rho v_0 v'_0
+          (* RV for recursive types *)
+          | Ty_IFix F T =>
+              exists v_0 v'_0 Fp Tp,
+                (* Determine the shape of e_f and e'_f *)
+                normalise Fp F /\ normalise Tp T /\
+                e_f = IWrap (msubstT (msyn1 rho) Fp) (msubstT (msyn1 rho) Tp) v_0 /\
+                e'_f = IWrap (msubstT (msyn2 rho) Fp) (msubstT (msyn2 rho) Tp) v'_0 /\
+                (* Unwrap *)
+                forall i (Hlt_i : i < k - j) K T0n,
+                  empty |-* (msubstT (msyn1 rho) T) : K ->
+                  empty |-* (msubstT (msyn2 rho) T) : K ->
+                  normalise (unwrapIFix F K T) T0n ->
+                  RC i T0n rho v_0 v'_0
 
-        (* RV for universal types *)
-        | Ty_Forall bX K T => 
-            (
+          (* RV for universal types *)
+          | Ty_Forall bX K T => 
               exists e_body e'_body,
                 (* Determine the shape of e_f and e_f' *)
                 e_f = TyAbs bX K e_body /\
@@ -161,61 +109,18 @@ Equations? RC (k : nat) (T : Ty) (rho : tymapping) (e e' : Term) : Prop by wf k 
                   Rel T1 T2 Chi ->
                   forall i (Hlt_i : i < k - j),
                     RC i T ((bX, (Chi, T1, T2)) :: rho) <{ [[T1 / bX ] e_body }> <{ [[T2 / bX ] e'_body }>
-            )
-      end.
+          end
+        ) \/ (
+          is_error e_f /\
+          is_error e'_f
+        )
+      ).
 Proof. all: lia. Qed.
 
 Definition RV (k : nat) (T : Ty) (rho : tymapping) (v v' : Term) : Prop :=
   value v /\ value v' /\ RC k T rho v v'.
 
-(** ** Helper lemmas for RC *)
-
-Lemma RV_typable_empty : forall k T rho v v',
-    RV k T rho v v' ->
-    0 < k ->
-    empty ,, empty |-+ v : (msubstT (msyn1 rho) T) /\ (empty ,, empty |-+ v' : (msubstT (msyn2 rho) T)).
-Proof. 
-  intros. 
-  unfold RV in H. 
-  destruct H as [Hval__v [Hval__v' HRC]].
-  autorewrite with RC in HRC.
-  apply eval_value in Hval__v as Hev__v.
-  unfold P_value in Hev__v.
-  apply HRC in Hev__v; auto.
-  clear HRC.
-  destruct Hev__v as [e'_f [j' [Hev__e'_f [Htyp__v [Htyp__v' _]]]]].
-  apply eval_value in Hval__v'.
-  assert (e'_f = v' /\ j' = 0) by (eapply eval__deterministic; eauto).
-  destruct H. subst.
-  auto.
-Qed.
-
-Lemma RV_typable_empty_1 : forall k T rho v v',
-    RV k T rho v v' ->
-    0 < k ->
-    empty ,, empty |-+ v : (msubstT (msyn1 rho) T).
-Proof. intros. destruct (RV_typable_empty _ _ _ _ _ H H0). eauto. Qed.
-
-Lemma RV_typable_empty_2 : forall k T rho v v',
-    RV k T rho v v' ->
-    0 < k ->
-    empty ,, empty |-+ v' : (msubstT (msyn2 rho) T).
-Proof. intros. destruct (RV_typable_empty _ _ _ _ _ H H0). eauto. Qed.
-
-Lemma RC_lt : forall k T rho e e',
-  (0 < k -> RC k T rho e e') ->
-  RC k T rho e e'.
-Proof.
-  intros.
-  autorewrite with RC.
-  intros j Hlt__j.
-  assert (0 < k) by lia.
-  apply H in H0.
-  autorewrite with RC in H0.
-  eapply H0.
-  assumption.
-Qed.
-
+(** Converting from RC to RV and vice versa *)
 
 Lemma RC_to_RV : forall k T rho e e',
     RC k T rho e e' ->
@@ -231,20 +136,19 @@ Proof.
   destruct temp as [e'_f [j' [Hev__e'_f [Htyp__e_f [Htyp__e'_f H]]]]].
   eexists. eexists.
   split. eauto.
-  split. eauto using eval_value, eval_to_value.
-  split. eauto using eval_value, eval_to_value.
+  split. eauto using eval_value__value, eval_to_value__eval.
+  split. eauto using eval_value__value, eval_to_value__eval.
   autorewrite with RC.
   intros.
   assert (e_f =[0]=> e_f). {
-    eapply eval_value.
-    eapply eval_to_value.
+    eapply eval_value__value.
+    eapply eval_to_value__eval.
     eauto.
   }
   assert (e_f0 = e_f /\ j0 = 0) by (eapply eval__deterministic; eauto).
   destruct H2. subst.
-  assert (forall i, i < k - 0 -> i < k - j) by apply skip.
   eexists. eexists.
-  split. eapply eval_value. eapply eval_to_value. eauto.
+  split. eapply eval_value__value. eapply eval_to_value__eval. eauto.
   rewrite <- minus_n_O.
   eauto.
 Qed.
@@ -259,764 +163,40 @@ Lemma RV_to_RC : forall k T rho v v',
   RC k T rho v v'.
 Proof. intros. apply H. Qed.
 
-Lemma RV_condition : forall k T rho v v',
-    RV k T rho v v' ->
-    0 < k ->
-
-    match T with
-
-        (* RV for type variable *)
-        | Ty_Var a =>
-            forall Chi,
-            sem rho a = Datatypes.Some Chi ->  
-            Chi k v v'
-
-        (* RV for type lambda *)
-        | Ty_Lam bX K T =>
-            False
-
-        (* RV for type application *)
-        | Ty_App T1 T2 => 
-            False
-
-        (* RV for built-in types *)
-        | Ty_Builtin st => 
-            exists sv sv',
-              (* Determine the shape of e_f and e'_f *)
-              v = Constant sv /\
-              v' = Constant sv' /\
-              (* Syntactic equality *)
-              v = v'
-
-        (* RV for function types *)
-        | Ty_Fun T1 T2 =>
-            (
-              (* Determine the shape of e_f and e'_f *)
-              exists x e_body x' e'_body,
-                LamAbs x (msubstT (msyn1 rho) T1) e_body = v /\
-                LamAbs x' (msubstT (msyn2 rho) T1) e'_body = v' /\
-                (* Extensional equivalence *)
-                forall i (Hlt_i : i < k) v_2 v'_2,
-                  RV i T1 rho v_2 v'_2 ->
-                  RC i T2 rho <{ [v_2 / x] e_body }> <{ [v'_2 / x'] e'_body }>
-            ) \/ (
-              (* Determine the shape of e_f and e'_f*)
-              exists f args f' args',
-                ExtBuiltin f args = v /\
-                ExtBuiltin f' args' = v' /\
-                (* Extensional equivalence*)
-                forall i (Hlt_i : i < k) v_0 v'_0,
-                  RV i T1 rho v_0 v'_0 ->
-                  RC i T2 rho (ExtBuiltin f (v_0 :: args)) (ExtBuiltin f' (v'_0 :: args'))
-            )
-
-        (* RV for recursive types *)
-        | Ty_IFix F T =>
-            exists v_2 v'_2,
-              (* Determine the shape of e_f and e_f' *)
-              v = IWrap (msubstT (msyn1 rho) F) (msubstT (msyn1 rho) T) v_2 /\
-              v' = IWrap (msubstT (msyn2 rho) F) (msubstT (msyn2 rho) T) v'_2 /\
-              (* Uwrap *)
-              forall i (Hlt_i : i < k) K S,
-                empty |-* (msubstT (msyn2 rho) T) : K ->
-                normalise (unwrapIFix F K T) S ->
-                RC i S rho v_2 v'_2
-
-        (* RV for universal types *)
-        | Ty_Forall bX K T => 
-            (
-              exists e_body e'_body,
-                (* Determine the shape of e_f and e_f' *)
-                v = TyAbs bX K e_body /\
-                v' = TyAbs bX K e'_body /\
-                (* Instantiational equivalence *)
-                forall T1 T2 Chi,
-                  empty |-* T1 : K ->
-                  empty |-* T2 : K ->
-                  Rel T1 T2 Chi ->
-                  forall i (Hlt_i : i < k),
-                    RC i T ((bX, (Chi, T1, T2)) :: rho) <{ [[T1 / bX ] e_body }> <{ [[T2 / bX ] e'_body }>
-            )
-      end.
-Proof.
-  intros.
-  destruct H as [Hval__v [Hval__v' HRC]].
-  apply eval_value in Hval__v as Hev__v.
-  unfold P_value in Hev__v.
-  apply eval_value in Hval__v' as Hev__v'.
-  unfold P_value in Hev__v'.
-  autorewrite with RC in HRC.
-  apply HRC in Hev__v as temp; eauto.
-  clear HRC.
-  destruct temp as [v'' [j'' [Hev__v'' [_ [_ condition]]]]].
-  assert (v'' = v' /\ j'' = 0) by (eapply eval__deterministic; eauto).
-  destruct H. subst.
-  rewrite <- minus_n_O in condition.
-  eauto. 
-Qed.
-  
-Corollary RV_syntactic_equality : forall k st rho v v',
-    RV k (Ty_Builtin st) rho v v' ->
-    0 < k ->
-
-    exists sv sv',
-      (* Determine the shape of e_f and e'_f *)
-      v = Constant sv /\
-      v' = Constant sv' /\
-      (* Syntactic equality *)
-      v = v'.
-Proof. intros. eapply RV_condition in H. all: eauto. Qed.
-
-Corollary RV_functional_extensionality : forall k T1 T2 rho v v',
-    RV k (Ty_Fun T1 T2) rho v v' ->
-    0 < k ->
-
-    (
-      exists x e_body x' e'_body,
-        (* Determine the shape of e_f and e'_f *)
-        LamAbs x (msubstT (msyn1 rho) T1) e_body = v /\
-        LamAbs x' (msubstT (msyn2 rho) T1) e'_body = v' /\
-        (* Extensional equivalence *)
-        forall i (Hlt_i : i < k) v_2 v'_2,
-          RV i T1 rho v_2 v'_2 ->
-          RC i T2 rho <{ [v_2 / x] e_body }> <{ [v'_2 / x'] e'_body }>
-    ) \/  (
-      (* Determine the shape of e_f and e'_f*)
-      exists f args f' args',
-        ExtBuiltin f args = v /\
-        ExtBuiltin f' args' = v' /\
-        (* Extensional equivalence*)
-        forall i (Hlt_i : i < k) v_0 v'_0,
-          RV i T1 rho v_0 v'_0 ->
-          RC i T2 rho (ExtBuiltin f (v_0 :: args)) (ExtBuiltin f' (v'_0 :: args'))
-    ).
-Proof. intros. eapply RV_condition in H. all: eauto. Qed.
-
-Corollary RV_unwrap : forall k F T rho v v' ,
-    RV k (Ty_IFix F T) rho v v' ->
-    0 < k ->
-
-    exists v_2 v'_2,
-      (* Determine the shape of e_f and e_f' *)
-      v = IWrap (msubstT (msyn1 rho) F) (msubstT (msyn1 rho) T) v_2 /\
-      v' = IWrap (msubstT (msyn2 rho) F) (msubstT (msyn2 rho) T) v'_2 /\
-      (* Uwrap *)
-      forall i (Hlt_i : i < k) K S,
-        empty |-* (msubstT (msyn2 rho) T) : K ->
-        normalise (unwrapIFix F K T) S ->
-        RC i S rho v_2 v'_2.
-Proof. intros. eapply RV_condition in H. all: eauto. Qed.
-
-Corollary RV_instantiational_extensionality : forall k bX K T rho v v',
-    RV k (Ty_Forall bX K T) rho v v' ->
-    0 < k ->
-
-    exists e_body e'_body,
-      (* Determine the shape of e_f and e_f' *)
-      v = TyAbs bX K e_body /\
-      v' = TyAbs bX K e'_body /\
-      (* Instantiational equivalence *)
-      forall T1 T2 Chi,
-        empty |-* T1 : K ->
-        empty |-* T2 : K ->
-        Rel T1 T2 Chi ->
-        forall i (Hlt_i : i < k),
-          RC i T ((bX, (Chi, T1, T2)) :: rho) <{ [[T1 / bX ] e_body }> <{ [[T2 / bX ] e'_body }>.
-Proof. intros. eapply RV_condition in H. all: eauto. Qed.
-
-
-(** ** Multisubstitutions, multi-extensions, and instantiations *)
-
+(** Kind assignments *)
 Definition kass := list (name * Kind).
 
+(** RD = Interpretation of kind contexts as type mappings *)
 Inductive RD : kass -> tymapping -> Prop :=
   | RD_nil :
       RD nil nil
   | RD_cons : forall ck rho T1 T2 Chi X K,
       empty |-* T1 : K ->
       empty |-* T2 : K ->
-      (* Something about the fact that T1 and T2 should be reduced? *)
       Rel T1 T2 Chi ->
       RD ck rho ->
       RD ((X, K) :: ck) ((X, (Chi, T1, T2)) :: rho).
 
-(** Instantiation *)
+(** Term environment *)
 Definition env := list (name * Term).
+(** Type assignments *)
 Definition tass := list (name * Ty).
 
+(** RG = Interpretation of type contexts as logically related term environments *)
 Inductive RG (rho : tymapping) (k : nat) : tass -> env -> env -> Prop :=
   | RG_nil :
       RG rho k nil nil nil
   | RG_cons : forall x T v1 v2 c e1 e2,
       RV k T rho (msubstA_term (msyn1 rho) v1) (msubstA_term (msyn2 rho) v2) ->
+      normal_Ty T ->
       RG rho k c e1 e2 ->
       RG rho k ((x, T) :: c) ((x, msubstA_term (msyn1 rho) v1) :: e1) ((x, msubstA_term (msyn2 rho) v2) :: e2).
   
-Fixpoint lookup {X:Type} (k : string) (l : list (name * X)) : option X :=
-  match l with
-  | nil => None
-  | (j,x) :: l' => if String.eqb j k then Datatypes.Some x else lookup k l'
-  end.
-
-Fixpoint drop {X:Type} (n:string) (nxs:list (string * X)) : list (string * X) :=
-  match nxs with
-  | nil => nil
-  | (n',x) :: nxs' => if String.eqb n' n then drop n nxs' else (n',x) :: (drop n nxs')
-  end.
-
-Fixpoint mdrop {X:Type} (ns : list string) (nxs: list (string * X)) : list (string * X) :=
-  match ns with
-  | nil => nxs
-  | n :: ns' =>
-      mdrop ns' (drop n nxs) 
-  end.
-
-Lemma subst_closed : forall t,
-    closed t -> 
-    forall x s,
-      <{ [s / x] t }> = t.
-Proof.
-  intros.
-  eapply vacuous_substitution; eauto.
-  unfold closed in H.
-  apply H.
-Qed.
-
-Lemma substA_closed : forall t,
-    closed t -> 
-    forall X T,
-      <{ [[T / X] t }> = t.
-Proof.
-  intros.
-  eapply vacuous_substituteA; eauto.
-  unfold closed in H.
-  apply H.
-Qed.
-
-Lemma subst_not_afi : forall t x v,
-    closed v ->
-    ~(appears_free_in_Term x <{ [v / x] t }> ).
-Proof.
-  unfold closed, not.
-  induction t; intros x v P A.
-  - simpl in A. destruct r.
-    + destruct (existsb (eqb x) (bvbs l)) eqn:Hexb.
-      * inversion A.
-        -- subst.
-Admitted.
-
-Lemma duplicate_subst : forall x t v v',
-    closed v ->
-    <{ [v' / x] ([v / x] t) }> = <{ [v / x] t }>.
-Proof. 
-  intros. eapply vacuous_substitution. apply subst_not_afi. assumption.
-Qed.
-
-Lemma duplicate__subst_bnr : forall x bs v v',
-    closed v ->
-    <{ [v' / x][bnr] ([v / x][bnr] bs) }> = <{ [v / x][bnr] bs }>.
-Proof. intros. Admitted.
-
-Lemma swap_subst : forall t x x1 v v1,
-    x <> x1 ->
-    closed v ->
-    closed v1 ->
-    <{ [v1/x1]([v/x]t) }> = <{ [v/x]([v1/x1]t) }>.
-Proof. Admitted.
-
-Lemma swap__subst_bnr : forall bs x x1 v v1,
-    x <> x1 ->
-    closed v ->
-    closed v1 ->
-    <{ [v1/x1][bnr]([v/x][bnr] bs) }> = <{ [v/x][bnr]([v1/x1][bnr] bs) }>.
-Proof. Admitted.
-
-
-
-(** ** Properties of multi-substitutions *)
-
-Lemma msubst_closed : forall t,
-    closed t ->
-    forall ss,
-       msubst_term ss t = t.
-Proof.
-  induction ss.
-  - reflexivity.
-  - destruct a.
-    simpl.
-    rewrite subst_closed; assumption.
-Qed.
-
-Lemma msubstA_closed : forall t,
-    closed t ->
-    forall ss,
-      msubstA_term ss t = t.
-Proof.
-  induction ss.
-  - reflexivity.
-  - destruct a.
-    simpl.
-    rewrite substA_closed; assumption.
-Qed.
-
 Fixpoint closed_env (env : env) :=
   match env with
   | nil => True
   | (x,t) :: env' => closed t /\ closed_env env'
   end.
-
-Fixpoint value_env (env : env) :=
-  match env with
-  | nil => True
-  | (x,t) :: env' => value t /\ value_env env'
-  end.
-
-Lemma subst_msubst : forall env x v t,
-    closed v ->
-    closed_env env ->
-    msubst_term env <{ [v/x]t }> = <{ [v/x] {msubst_term (drop x env) t} }>.
-Proof.
-  induction env0; intros; auto.
-  destruct a. simpl.
-  inversion H0.
-  destruct (s =? x) eqn:Heqb.
-  - apply eqb_eq in Heqb as Heq.
-    subst.
-    rewrite duplicate_subst; auto.
-  - apply eqb_neq in Heqb as Hneq.
-    rewrite swap_subst; eauto.
-Qed.
-
-Lemma subst_msubst' : forall env x v t,
-    closed v ->
-    closed_env env ->
-    msubst_term (drop x env) <{ [v/x]t }> = <{ [v/x] {msubst_term (drop x env) t} }>.
-Proof.
-  induction env0; intros; auto.
-  destruct a. simpl.
-  inversion H0.
-  destruct (s =? x) eqn:Heqb.
-  - apply eqb_eq in Heqb as Heq.
-    subst.
-    eauto.
-  - apply eqb_neq in Heqb as Hneq.
-    simpl.  
-    rewrite swap_subst; eauto.
-Qed.
-
-Lemma subst_msubst'' : forall env x xs v t,
-    closed v ->
-    closed_env env ->
-    ~ In x xs ->
-    msubst_term (mdrop xs env) <{ [v/x]t }> = <{ [v/x] {msubst_term (mdrop xs env) t} }>.
-Proof. Admitted.
-
-Lemma subst_bnr__msubst_bnr : forall env x v bs,
-    closed v ->
-    closed_env env ->
-    msubst_bindings_nonrec env <{ [v/x][bnr] bs }> = <{ [v/x][bnr] {msubst_bindings_nonrec (drop x env) bs} }>.
-Proof.
-  induction env0; intros; auto.
-  destruct a. simpl.
-  inversion H0.
-  destruct (s =? x) eqn:Heqb.
-  - apply eqb_eq in Heqb as Heq.
-    subst.
-    rewrite duplicate__subst_bnr; auto.
-  - apply eqb_neq in Heqb as Hneq.
-    rewrite swap__subst_bnr; eauto.
-Qed.
-
-Lemma subst_bnr__msubst_bnr' : forall env x v bs,
-    closed v ->
-    closed_env env ->
-    msubst_bindings_nonrec (drop x env) <{ [v/x][bnr] bs }> = <{ [v/x][bnr] {msubst_bindings_nonrec (drop x env) bs} }>.
-Proof. Admitted.
-Lemma substA_msubstA : forall envA X U t,
-    closed_Ty U ->
-    msubstA_term envA <{ [[U/X]t }> = <{ [[U/X] {msubstA_term (drop X envA) t} }>.
-Proof. Admitted.
-
-(** ** Properties of multi-extensions *)
-
-Lemma mupdate_lookup : forall (c : tass) (x : name),
-    lookup x c = (mupdate empty c) x.
-Proof.
-  induction c.
-  - intros.
-    simpl.
-    reflexivity.
-  - intros.
-    simpl.
-    destruct a.
-    destruct (s =? x) eqn:Heqb.
-    + apply eqb_eq in Heqb as Heq.
-      subst.
-      rewrite update_eq.
-      reflexivity.
-    + apply eqb_neq in Heqb as Hneq.
-      rewrite update_neq; auto.
-Qed.
-
-Lemma mupdate_drop : forall (c : tass) x T,
-    (x |-> T; mupdate empty c) = (x |-> T; mupdate empty (drop x c)).
-Proof. 
-  induction c; intros. 
-  - auto.
-  - destruct a.
-    simpl.
-    destruct (s =? x) eqn:Heqb.
-    + apply eqb_eq in Heqb as Heq.
-      subst.
-      rewrite update_shadow.
-      auto.
-    + apply eqb_neq in Heqb as Hneq.
-      rewrite update_permute; auto.
-      simpl.
-      assert ((x |-> T; s |-> t; mupdate empty (drop x c)) = (s |-> t; x |-> T; mupdate empty (drop x c))). {
-        apply update_permute. auto. 
-      }
-      rewrite H.
-      f_equal.
-      auto.
-Qed.
-
-(*
-Lemma mupdate_drop : forall (c : tass) Gamma x x',
-      lookupT (mupdate Gamma (drop x c)) x' 
-    = if String.eqb x x' 
-        then lookupT Gamma x' 
-        else lookupT (mupdate Gamma c) x'.
-Proof. Admitted.
-*)
-
-Lemma mupdate_unfold : forall {X : Type} (c : list (string * X)) x (v : X),
-    (x |-> v; mupdate empty c) = mupdate empty ((x, v) :: c).
-Proof. intros. auto. Qed.
-
-Lemma mdrop_nil : forall X ns,
-    @mdrop X ns nil = nil.
-Proof. induction ns; auto. Qed.
-
-(** ** Properties of Instantiations *)
-
-Lemma RD_rel : forall ck rho,
-    RD ck rho ->
-    forall X Chi T1 T2,
-      sem rho X = Datatypes.Some Chi ->
-      syn1 rho X = Datatypes.Some T1 ->
-      syn2 rho X = Datatypes.Some T2 ->
-      Rel T1 T2 Chi.
-Proof.
-  induction 1.
-  - intros.
-    unfold sem in H.
-    inversion H.
-  - intros.
-    unfold sem in H3.
-    unfold syn1 in H4.
-    unfold syn2 in H5.
-    destruct (X0 =? X) eqn:Heqb.
-    + inversion H3. subst.
-      inversion H4. subst.
-      inversion H5. subst.
-      assumption.
-    + fold sem in H3.
-      fold syn1 in H4.
-      fold syn2 in H5.
-      eapply IHRD; eauto.
-Qed.
-
-Lemma RD_sem_syn : forall ck rho,
-    RD ck rho ->
-    forall X Chi,
-      sem rho X = Datatypes.Some Chi ->
-      exists T1 T2, 
-        syn1 rho X = Datatypes.Some T1 /\
-        syn2 rho X = Datatypes.Some T2.
-Proof.
-  induction 1.
-  - intros.
-    unfold sem in H.
-    inversion H.
-  - intros.
-    unfold sem in H3.
-    simpl.
-    destruct (X0 =? X) eqn:Heqb; eauto.
-Qed.
-
-Lemma RG_extend_rho : forall X Chi T1 T2 rho k c env env' ,
-    RG rho k c env env' ->
-    RG ((X, (Chi, T1, T2)) :: rho) k c env env'.
-Proof. Admitted.
-
-Lemma RG_domains_match : forall c e1 e2 k rho,
-    RG rho k c e1 e2 ->
-    forall x T,
-      lookup x c = Datatypes.Some T ->
-      exists v1 v2,
-        lookup x e1 = Datatypes.Some v1 /\
-        lookup x e2 = Datatypes.Some v2.
-Proof.
-  intros c e1 e2 k rho V. 
-  induction V; intros x0 T0 C.
-  - discriminate.
-  - simpl.
-    simpl in C.
-    destruct (x =? x0) eqn:Heqb.
-    + exists (msubstA_term (msyn1 rho) v1), (msubstA_term (msyn2 rho) v2). split; auto.
-    + apply IHV with T0.
-      assumption.
-Qed.
-
-Lemma RG_env_closed : forall rho k c e1 e2,
-    RG rho k c e1 e2 ->
-    0 < k ->
-    closed_env e1 /\ closed_env e2.
-Proof.
-  intros rho k c e1 e2 V Hlt.
-  induction V; intros.
-  - split; reflexivity.
-  - split.
-    + simpl.
-      split.
-      * eapply typable_empty__closed.
-        eapply RV_typable_empty_1 in H; eauto.
-      * apply IHV.
-    + simpl.
-      split.
-      * eapply typable_empty__closed.
-        eapply RV_typable_empty_2 in H; eauto.
-    * apply IHV.
-Qed.
-
-Corollary RG_env_closed_1 : forall rho k c e1 e2,
-    RG rho k c e1 e2 ->
-    0 < k ->
-    closed_env e1.
-Proof. intros. destruct (RG_env_closed _ _ _ _ _ H H0). assumption. Qed.
-
-Corollary RG_env_closed_2 : forall rho k c e1 e2,
-    RG rho k c e1 e2 ->
-    0 < k ->
-    closed_env e2.
-Proof. intros. destruct (RG_env_closed _ _ _ _ _ H H0). assumption. Qed.
-
-Lemma RG_env_values : forall rho k c e1 e2,
-    RG rho k c e1 e2 ->
-    value_env e1 /\ value_env e2.
-Proof.
-  intros rho k c e1 e2 V.
-  induction V; intros.
-  - split; reflexivity.
-  - split.
-    + simpl.
-      split.
-      * eapply H.
-      * apply IHV. 
-    + split.
-      * eapply H.
-      * apply IHV.  
-Qed.
-
-Lemma RG_env_values_1 : forall rho k c e1 e2,
-    RG rho k c e1 e2 ->
-    value_env e1.
-Proof. intros. destruct (RG_env_values _ _ _ _ _ H). assumption. Qed.
-
-Lemma RG_env_values_2 : forall rho k c e1 e2,
-    RG rho k c e1 e2 ->
-    value_env e2.
-Proof. intros. destruct (RG_env_values _ _ _ _ _ H). assumption. Qed. 
-
-Lemma RG_RV : forall rho k c e1 e2,
-    RG rho k c e1 e2 ->
-    forall x T v1 v2,
-      lookup x c = Datatypes.Some T ->
-      lookup x e1 = Datatypes.Some v1 ->
-      lookup x e2 = Datatypes.Some v2 ->
-      RV k T rho v1 v2.
-Proof.
-  intros rho k c e1 e2 V.
-  induction V; intros x' T' v1' v2' G E1 E2.
-  - destruct x'; discriminate.
-  - inversion G. subst.
-    inversion E1. subst.
-    inversion E2. subst.
-    destruct (x =? x').
-    + inversion H1. subst.
-      inversion H2. subst.
-      inversion H3. subst.
-      assumption. 
-    + apply IHV with x'; assumption.
-Qed.
-
-Lemma RG_drop : forall rho k c e1 e2,
-    RG rho k c e1 e2 ->
-    forall x,
-      RG rho k (drop x c) (drop x e1) (drop x e2).
-Proof.
-  intros rho k c e1 e2 V.
-  induction V.
-  - intros. simpl. apply RG_nil.
-  - intros. simpl.
-    destruct (x =? x0).
-    + apply IHV.
-    + eapply RG_cons.
-      * eassumption.
-      * apply IHV.
-Qed.
-
-(** ** Congruence lemmas on [eval] *)
-
-(** ** Multi-substitutions preserve typing *)
-
-Fixpoint mupd (xts : tass) (Gamma : Gamma) : Implementations.Gamma :=
-  match xts with
-  | nil => Gamma
-  | ((a, T) :: xts') => mupd xts' (upd a T Gamma)
-  end.
-
-Lemma mupd_nil : forall Gamma,
-    mupd nil Gamma = Gamma.
-Proof. intros. apply Coq.Logic.FunctionalExtensionality.functional_extensionality. intros. unfold mupd. destruct (Gamma x); auto. Qed.
-
-Lemma mupd_absorbs_msubstT : forall xts x T Gamma,
-    mupd xts (x |-> T; Gamma) = (x |-> msubstT xts T; mupd xts Gamma).
-Proof.
-  induction xts.
-  - auto.
-  - intros.
-    destruct a. 
-    simpl.
-    rewrite <- upd_absorbs_substituteT.
-    eauto.
-Qed.
-
-Lemma mupd_empty : forall xts,
-    mupd xts empty = empty.
-Proof. induction xts; auto. simpl. destruct a. auto. Qed.
-
-Lemma msubstA_preserves_typing_1 : forall rho ck,
-    RD ck rho ->
-    forall Delta Gamma t T,
-      mupdate Delta ck ,, Gamma |-+ t : T ->
-      Delta ,, mupd (msyn1 rho) Gamma |-+ (msubstA_term (msyn1 rho) t) : (msubstT (msyn1 rho) T). 
-Proof.
-  intros rho ck V.
-  induction V.
-  - intros.
-    subst.
-    simpl.
-    assumption.
-  - intros.
-    subst.
-    simpl.
-    unfold mupd.
-    simpl.
-    eapply IHV; eauto.
-    eapply substituteA_preserves_typing; eauto.
-Qed.
-
-Lemma msubstA_preserves_typing_2 : forall rho ck,
-    RD ck rho ->
-    forall Delta Gamma t T,
-      mupdate Delta ck ,, Gamma |-+ t : T ->
-      Delta ,, mupd (msyn2 rho) Gamma |-+ (msubstA_term (msyn2 rho) t) : (msubstT (msyn2 rho) T). 
-Proof.
-  intros rho ck V.
-  induction V.
-  - intros.
-    subst.
-    simpl.
-    assumption.
-  - intros.
-    subst.
-    simpl.
-    unfold mupd.
-    simpl.
-    eapply IHV; eauto.
-    eapply substituteA_preserves_typing; eauto.
-Qed.
-
-Lemma msubst_preserves_typing_1 : forall rho k c e1 e2,
-    RG rho k c e1 e2 ->
-    0 < k ->
-    forall Gamma T t,
-      empty ,, (mupd (msyn1 rho) (mupdate Gamma c)) |-+ t : (msubstT (msyn1 rho) T) ->
-      empty ,, (mupd (msyn1 rho) Gamma) |-+ (msubst_term e1 t) : (msubstT (msyn1  rho) T). 
-Proof.
-  intros rho k c e1 e2 V Hlt.
-  induction V.
-  - intros.
-    simpl.
-    assumption.
-  - intros.
-    eapply IHV.
-    eapply substitution_preserves_typing.
-    + simpl in H0.
-      rewrite mupd_absorbs_msubstT in H0.
-      eauto.
-    + eapply RV_typable_empty_1 in H.
-      eauto.
-      eauto.
-Qed. 
-
-Lemma msubst_preserves_typing_2 : forall rho k c e1 e2,
-    RG rho k c e1 e2 ->
-    0 < k ->
-    forall Gamma T t,
-      empty ,, (mupd (msyn2 rho) (mupdate Gamma c)) |-+ t : (msubstT (msyn2 rho) T) ->
-      empty ,, (mupd (msyn2 rho) Gamma) |-+ (msubst_term e2 t) : (msubstT (msyn2 rho) T). 
-Proof.
-  intros rho k c e1 e2 V Hlt.
-  induction V.
-  - intros.
-    simpl.
-    assumption.
-  - intros.
-    eapply IHV.
-    eapply substitution_preserves_typing.
-    + simpl in H0.
-      rewrite mupd_absorbs_msubstT in H0.
-      eauto.
-    + eapply RV_typable_empty_2 in H.
-      eauto.
-      eauto.
-Qed. 
-
-Lemma msubstT_preserves_kinding_1 : forall ck rho,
-  RD ck rho ->
-  forall Delta T K,
-    (mupdate Delta ck) |-* T : K ->
-    Delta |-* (msubstT (msyn1 rho) T) : K.
-Proof.
-  intros ck rho V.
-  induction V; intros.
-  - assumption.
-  - simpl.
-    eapply IHV.
-    eapply substituteT_preserves_kinding.
-    + apply H2.
-    + assumption.
-Qed.
-
-Lemma msubstT_preserves_kinding_2 : forall ck rho,
-  RD ck rho ->
-  forall Delta T K,
-    (mupdate Delta ck) |-* T : K ->
-    Delta |-* (msubstT (msyn2 rho) T) : K.
-Proof.
-  intros ck rho V.
-  induction V; intros.
-  - assumption.
-  - simpl.
-    eapply IHV.
-    eapply substituteT_preserves_kinding.
-    + apply H2.
-    + assumption.
-Qed.
-
 
 (** Logical relation: logical approximation
 
@@ -1047,8 +227,8 @@ Definition LR_logically_equivalent (Delta : partial_map Kind) (Gamma : partial_m
   LR_logically_approximate Delta Gamma e e' T /\ LR_logically_approximate Delta Gamma e' e T.
 
 Definition LR_logically_approximate_binding (Delta : Delta) (Gamma : Gamma) (b b' : Binding) :=
-  Delta ,, Gamma |-ok b /\
-  (Delta ,, Gamma |-ok b') /\
+  Delta ,, Gamma |-ok_b b /\
+  (Delta ,, Gamma |-ok_b b') /\
   match b, b' with
   | TermBind s (VarDecl x T) e, TermBind s' (VarDecl x' T') e' =>
       s' = s /\
