src/Language/PlutusIR/Semantics/SemanticEquivalence/Auto.v
@@ -1,6 +1,6 @@
 Require Import PlutusCert.Language.PlutusIR.Semantics.Static.
 Require Import PlutusCert.Language.PlutusIR.Semantics.Dynamic.
-Require Import PlutusCert.Language.PlutusIR.Semantics.SemanticEquivalence.LogicalRelation.RelationalModel.
+Require Import PlutusCert.Language.PlutusIR.Semantics.SemanticEquivalence.LogicalRelation.
 
 From Coq Require Import Lia.
 
@@ -9,20 +9,20 @@ Ltac multisubst_preserves_typing :=
   | |- 
       empty ,, empty |-+ (msubst_term ?env (msubstA_term (msyn1 ?rho) ?e)) : (msubstT (msyn1 ?rho) ?T)
     => 
-      replace empty with (mupd (msyn1 rho) empty);
+      replace empty with (mgsubst (msyn1 rho) empty);
         [ eapply msubst_preserves_typing_1; eauto;
           eapply msubstA_preserves_typing_1; eauto;
           eauto with typing
-        | rewrite mupd_empty; reflexivity
+        | rewrite mgsubst_empty; reflexivity
         ]
   | |- 
       empty ,, empty |-+ (msubst_term ?env (msubstA_term (msyn2 ?rho) ?e)) : (msubstT (msyn2 ?rho) ?T)
     => 
-      replace empty with (mupd (msyn2 rho) empty);
+      replace empty with (mgsubst (msyn2 rho) empty);
         [ eapply msubst_preserves_typing_2; eauto;
           eapply msubstA_preserves_typing_2; eauto;
           eauto with typing
-        | rewrite mupd_empty; reflexivity
+        | rewrite mgsubst_empty; reflexivity
         ]
   end.
   
