src/Language/PlutusIR/Semantics/SemanticEquivalence/LogicalRelation.v
@@ -1,0 +1,8 @@
+Require Export PlutusCert.Language.PlutusIR.Semantics.SemanticEquivalence.LogicalRelation.Monotonicity.
+Require Export PlutusCert.Language.PlutusIR.Semantics.SemanticEquivalence.LogicalRelation.RelationalModel.
+Require Export PlutusCert.Language.PlutusIR.Semantics.SemanticEquivalence.LogicalRelation.Tymapping.
+Require Export PlutusCert.Language.PlutusIR.Semantics.SemanticEquivalence.LogicalRelation.RC.Helpers.
+Require Export PlutusCert.Language.PlutusIR.Semantics.SemanticEquivalence.LogicalRelation.RD.Helpers.
+Require Export PlutusCert.Language.PlutusIR.Semantics.SemanticEquivalence.LogicalRelation.RG.Helpers.
+Require Export PlutusCert.Language.PlutusIR.Semantics.SemanticEquivalence.LogicalRelation.RV.Helpers.
+Require Export PlutusCert.Language.PlutusIR.Semantics.SemanticEquivalence.LogicalRelation.Subst.
