src/Language/PlutusIR/Semantics/SemanticEquivalence/LogicalRelation/RD/Helpers.v
@@ -1,0 +1,53 @@
+Require Import PlutusCert.Language.PlutusIR.Semantics.Static.
+Require Import PlutusCert.Language.PlutusIR.Semantics.Dynamic.
+Require Import PlutusCert.Language.PlutusIR.Semantics.SemanticEquivalence.LogicalRelation.Tymapping.
+Require Import PlutusCert.Language.PlutusIR.Semantics.SemanticEquivalence.LogicalRelation.RelationalModel.
+
+Local Open Scope string_scope.
+
+
+
+Lemma RD_Rel : forall ck rho,
+    RD ck rho ->
+    forall X Chi T1 T2,
+      sem rho X = Datatypes.Some Chi ->
+      syn1 rho X = Datatypes.Some T1 ->
+      syn2 rho X = Datatypes.Some T2 ->
+      Rel T1 T2 Chi.
+Proof.
+  induction 1.
+  - intros.
+    unfold sem in H.
+    inversion H.
+  - intros.
+    unfold sem in H3.
+    unfold syn1 in H4.
+    unfold syn2 in H5.
+    destruct (X0 =? X) eqn:Heqb.
+    + inversion H3. subst.
+      inversion H4. subst.
+      inversion H5. subst.
+      assumption.
+    + fold sem in H3.
+      fold syn1 in H4.
+      fold syn2 in H5.
+      eapply IHRD; eauto.
+Qed.
+
+Lemma RD_sem_syn : forall ck rho,
+    RD ck rho ->
+    forall X Chi,
+      sem rho X = Datatypes.Some Chi ->
+      exists T1 T2, 
+        syn1 rho X = Datatypes.Some T1 /\
+        syn2 rho X = Datatypes.Some T2.
+Proof.
+  induction 1.
+  - intros.
+    unfold sem in H.
+    inversion H.
+  - intros.
+    unfold sem in H3.
+    simpl.
+    destruct (X0 =? X) eqn:Heqb; eauto.
+Qed.
