src/Language/PlutusIR/Semantics/SemanticEquivalence/LogicalRelation/RV/Helpers.v
@@ -1,0 +1,236 @@
+Require Import PlutusCert.Language.PlutusIR.Semantics.Static.
+Require Import PlutusCert.Language.PlutusIR.Semantics.Dynamic.
+Require Import PlutusCert.Language.PlutusIR.Semantics.SemanticEquivalence.LogicalRelation.Tymapping.
+Require Import PlutusCert.Language.PlutusIR.Semantics.SemanticEquivalence.LogicalRelation.RelationalModel.
+
+From Coq Require Import Arith.
+
+Local Open Scope list_scope.
+
+
+
+(** Empty typability *)
+
+Lemma RV_typable_empty : forall k T rho v v',
+    RV k T rho v v' ->
+    0 < k ->
+    (exists Tn, normalise (msubstT (msyn1 rho) T) Tn /\ (empty ,, empty |-+ v : Tn)) /\
+    (exists Tn', normalise (msubstT (msyn2 rho) T) Tn' /\  (empty ,, empty |-+ v' : Tn')).
+Proof. 
+  intros. 
+  unfold RV in H. 
+  destruct H as [Hval__v [Hval__v' HRC]].
+  autorewrite with RC in HRC.
+  apply eval_value in Hval__v as Hev__v.
+  apply HRC in Hev__v; auto.
+  clear HRC.
+  destruct Hev__v as [e'_f [j' [Hev__e'_f [Htyp__v [Htyp__v' _]]]]].
+  apply eval_value in Hval__v'.
+  assert (e'_f = v' /\ j' = 0) by (eapply eval__deterministic; eauto).
+  destruct H. subst.
+  auto.
+Qed.
+
+Lemma RV_typable_empty_1 : forall k T rho v v',
+    RV k T rho v v' ->
+    0 < k ->
+    (exists Tn, normalise (msubstT (msyn1 rho) T) Tn /\ (empty ,, empty |-+ v : Tn)).
+Proof. intros. destruct (RV_typable_empty _ _ _ _ _ H H0) as [Htyp__v Htyp__v']. eauto. Qed.
+
+Lemma RV_typable_empty_2 : forall k T rho v v',
+    RV k T rho v v' ->
+    0 < k ->
+    (exists Tn', normalise (msubstT (msyn2 rho) T) Tn' /\ (empty ,, empty |-+ v' : Tn')).
+Proof. intros. destruct (RV_typable_empty _ _ _ _ _ H H0) as [Htyp__v Htyp__v']. eauto. Qed.
+
+(** Equivalnce of step-index implies equivalence of RV *)
+
+Lemma RV_equiv : forall k k' T rho e e',
+    RV k T rho e e' ->
+    k = k' ->
+    RV k' T rho e e'.
+Proof. intros. subst. eauto. Qed.
+
+(** Easy access to the RV conditions *)
+
+Lemma RV_condition : forall k T rho v v',
+    RV k T rho v v' ->
+    0 < k ->
+
+    ( 
+      ~ is_error v /\
+      ~ is_error v' /\
+      (
+        match T with
+
+        (* RV for type variable *)
+        | Ty_Var a =>
+            forall Chi,
+              sem rho a = Datatypes.Some Chi ->  
+              Chi k v v'
+
+        (* RV for type lambda *)
+        | Ty_Lam bX K T =>
+            False
+
+        (* RV for type application *)
+        | Ty_App T1 T2 => 
+            False
+
+        (* RV for built-in types *)
+        | Ty_Builtin st => 
+            exists sv sv',
+              (* Determine the shape of v and v'*)
+              v = Constant sv /\
+              v' = Constant sv' /\
+              (* Syntactic equality *)
+              v = v'
+
+        (* RV for function types *)
+        | Ty_Fun T1 T2 =>
+            (* Determine the shape of v and v' *)
+            exists x e_body x' e'_body T1p,
+              normalise T1p T1 /\   
+              LamAbs x (msubstT (msyn1 rho) T1p) e_body = v /\
+              LamAbs x' (msubstT (msyn2 rho) T1p) e'_body = v' /\
+              (* Extensional equivalence *)
+              forall i (Hlt_i : i < k) v_0 v'_0,
+                value v_0 /\ value v'_0 /\ RC i T1 rho v_0 v'_0 ->
+                RC i T2 rho <{ [v_0 / x] e_body }> <{ [v'_0 / x'] e'_body }>
+
+        (* RV for recursive types *)
+        | Ty_IFix F T =>
+            exists v_0 v'_0 Fp Tp,
+              (* Determine the shape of v and v' *)
+              normalise Fp F /\ normalise Tp T /\
+              v = IWrap (msubstT (msyn1 rho) Fp) (msubstT (msyn1 rho) Tp) v_0 /\
+              v' = IWrap (msubstT (msyn2 rho) Fp) (msubstT (msyn2 rho) Tp) v'_0 /\
+              (* Unwrap *)
+              forall i (Hlt_i : i < k) K T0n,
+                empty |-* (msubstT (msyn1 rho) T) : K ->
+                empty |-* (msubstT (msyn2 rho) T) : K ->
+                normalise (unwrapIFix F K T) T0n ->
+                RC i T0n rho v_0 v'_0
+
+        (* RV for universal types *)
+        | Ty_Forall bX K T => 
+            exists e_body e'_body,
+              (* Determine the shape of v and v' *)
+              v = TyAbs bX K e_body /\
+              v' = TyAbs bX K e'_body /\
+              (* Instantiational equivalence *)
+              forall T1 T2 Chi,
+                empty |-* T1 : K ->
+                empty |-* T2 : K ->
+                Rel T1 T2 Chi ->
+                forall i (Hlt_i : i < k),
+                  RC i T ((bX, (Chi, T1, T2)) :: rho) <{ [[T1 / bX ] e_body }> <{ [[T2 / bX ] e'_body }>
+        end
+      ) \/ (
+        is_error v /\
+        is_error v'
+      )
+    ).
+Proof.
+  intros.
+  destruct H as [Hval__v [Hval__v' HRC]].
+  apply eval_value__value in Hval__v as Hev__v.
+  apply eval_value__value in Hval__v' as Hev__v'.
+  autorewrite with RC in HRC.
+  apply HRC in Hev__v as temp; eauto.
+  clear HRC.
+  destruct temp as [v'' [j'' [Hev__v'' [_ [_ condition]]]]].
+  assert (v'' = v' /\ j'' = 0) by (eapply eval__deterministic; eauto).
+  destruct H. subst.
+  rewrite <- minus_n_O in condition.
+  eauto. 
+Qed.
+  
+Corollary RV_syntactic_equality : forall k st rho v v',
+    RV k (Ty_Builtin st) rho v v' ->
+    0 < k ->
+
+    ( 
+      ~ is_error v /\
+      ~ is_error v' /\
+      exists sv sv',
+        (* Determine the shape of v and v' *)
+        v = Constant sv /\
+        v' = Constant sv' /\
+        (* Syntactic equality *)
+        v = v'
+    ) \/ (
+      is_error v /\
+      is_error v'
+    ).
+Proof. intros. eapply RV_condition in H. all: eauto. Qed.
+
+Corollary RV_functional_extensionality : forall k T1 T2 rho v v',
+    RV k (Ty_Fun T1 T2) rho v v' ->
+    0 < k ->
+
+    ( 
+      ~ is_error v /\
+      ~ is_error v' /\
+      (* Determine the shape of v and v' *)
+      exists x e_body x' e'_body T1p,
+        normalise T1p T1 /\   
+        LamAbs x (msubstT (msyn1 rho) T1p) e_body = v /\
+        LamAbs x' (msubstT (msyn2 rho) T1p) e'_body = v' /\
+        (* Extensional equivalence *)
+        forall i (Hlt_i : i < k) v_0 v'_0,
+          value v_0 /\ value v'_0 /\ RC i T1 rho v_0 v'_0 ->
+          RC i T2 rho <{ [v_0 / x] e_body }> <{ [v'_0 / x'] e'_body }>
+    ) \/ (
+      is_error v /\
+      is_error v'
+    ).
+Proof. intros. eapply RV_condition in H. all: eauto. Qed.
+
+Corollary RV_unwrap : forall k F T rho v v' ,
+    RV k (Ty_IFix F T) rho v v' ->
+    0 < k ->
+
+    (
+      ~ is_error v /\
+      ~ is_error v' /\
+      exists v_0 v'_0 Fp Tp,
+        (* Determine the shape of v and v' *)
+        normalise Fp F /\ normalise Tp T /\
+        v = IWrap (msubstT (msyn1 rho) Fp) (msubstT (msyn1 rho) Tp) v_0 /\
+        v' = IWrap (msubstT (msyn2 rho) Fp) (msubstT (msyn2 rho) Tp) v'_0 /\
+        (* Unwrap *)
+        forall i (Hlt_i : i < k) K T0n,
+          empty |-* (msubstT (msyn1 rho) T) : K ->
+          empty |-* (msubstT (msyn2 rho) T) : K ->
+          normalise (unwrapIFix F K T) T0n ->
+          RC i T0n rho v_0 v'_0
+    ) \/ (
+      is_error v /\
+      is_error v'
+    ).
+Proof. intros. eapply RV_condition in H. all: eauto. Qed.
+
+Corollary RV_instantiational_extensionality : forall k bX K T rho v v',
+    RV k (Ty_Forall bX K T) rho v v' ->
+    0 < k ->
+
+    (
+      ~ is_error v /\
+      ~ is_error v' /\
+      exists e_body e'_body,
+        (* Determine the shape of v and v' *)
+        v = TyAbs bX K e_body /\
+        v' = TyAbs bX K e'_body /\
+        (* Instantiational equivalence *)
+        forall T1 T2 Chi,
+          empty |-* T1 : K ->
+          empty |-* T2 : K ->
+          Rel T1 T2 Chi ->
+          forall i (Hlt_i : i < k),
+            RC i T ((bX, (Chi, T1, T2)) :: rho) <{ [[T1 / bX ] e_body }> <{ [[T2 / bX ] e'_body }>
+    ) \/ (
+      is_error v /\
+      is_error v'
+    ).
+Proof. intros. eapply RV_condition in H. all: eauto. Qed.
