src/Language/PlutusIR/Semantics/SemanticEquivalence/LogicalRelation/Subst.v
@@ -1,0 +1,414 @@
+Require Import PlutusCert.Language.PlutusIR.Semantics.Static.
+Require Import PlutusCert.Language.PlutusIR.Semantics.Dynamic.
+Require Import PlutusCert.Language.PlutusIR.Semantics.SemanticEquivalence.LogicalRelation.RelationalModel.
+Require Import PlutusCert.Language.PlutusIR.Semantics.SemanticEquivalence.LogicalRelation.Tymapping.
+Require Import PlutusCert.Language.PlutusIR.Semantics.SemanticEquivalence.LogicalRelation.RC.Helpers.
+Require Import PlutusCert.Language.PlutusIR.Semantics.SemanticEquivalence.LogicalRelation.RD.Helpers.
+Require Import PlutusCert.Language.PlutusIR.Semantics.SemanticEquivalence.LogicalRelation.RG.Helpers.
+Require Import PlutusCert.Language.PlutusIR.Semantics.SemanticEquivalence.LogicalRelation.RV.Helpers.
+Require Import PlutusCert.Language.PlutusIR.Semantics.TypeSafety.SubstitutionPreservesTyping.
+Require Import PlutusCert.Util.Map.Mupdate.
+Require Import PlutusCert.Util.List.
+
+Require Import Coq.Lists.List.
+
+Local Open Scope string_scope.
+
+
+
+(** Properties of substitutions *)
+
+Lemma subst_closed : forall t,
+    closed t -> 
+    forall x s,
+      <{ [s / x] t }> = t.
+Proof. Admitted.
+
+Lemma substA_closed : forall t,
+    closed t -> 
+    forall X T,
+      <{ [[T / X] t }> = t.
+Proof. Admitted.
+
+Lemma subst_not_afi : forall t x v,
+    closed v ->
+    ~(Term.appears_free_in x <{ [v / x] t }> ).
+Proof. Admitted.
+
+Lemma substA_not_afi : forall t X U,
+    Ty.closed U ->
+    ~(Annotation.appears_free_in X <{ [[U / X] t }> ).
+Proof. Admitted.
+
+Lemma duplicate_subst : forall x t v v',
+    closed v ->
+    <{ [v' / x] ([v / x] t) }> = <{ [v / x] t }>.
+Proof. Admitted.
+
+Lemma duplicate_substA : forall X t U U',
+    Ty.closed U ->
+    <{ [[U' / X] ([[U / X] t) }> = <{ [[U / X] t }>.
+Proof. Admitted.
+
+Lemma duplicate__subst_bnr : forall x bs v v',
+    closed v ->
+    <{ [v' / x][bnr] ([v / x][bnr] bs) }> = <{ [v / x][bnr] bs }>.
+Proof. Admitted.
+
+Lemma swap_subst : forall t x x1 v v1,
+    x <> x1 ->
+    closed v ->
+    closed v1 ->
+    <{ [v1/x1]([v/x]t) }> = <{ [v/x]([v1/x1]t) }>.
+Proof. Admitted.
+
+Lemma swap__subst_bnr : forall bs x x1 v v1,
+    x <> x1 ->
+    closed v ->
+    closed v1 ->
+    <{ [v1/x1][bnr]([v/x][bnr] bs) }> = <{ [v/x][bnr]([v1/x1][bnr] bs) }>.
+Proof. Admitted.
+
+
+
+(** ** Properties of multi-substitutions *)
+
+Lemma msubst_closed : forall t,
+    closed t ->
+    forall ss,
+       msubst_term ss t = t.
+Proof.
+  induction ss.
+  - reflexivity.
+  - destruct a.
+    simpl.
+    rewrite subst_closed; assumption.
+Qed.
+
+Lemma msubstA_closed : forall t,
+    closed t ->
+    forall ss,
+      msubstA_term ss t = t.
+Proof.
+  induction ss.
+  - reflexivity.
+  - destruct a.
+    simpl.
+    rewrite substA_closed; assumption.
+Qed.
+
+Lemma subst_msubst : forall env x v t,
+    closed v ->
+    closed_env env ->
+    msubst_term env <{ [v/x]t }> = <{ [v/x] {msubst_term (drop x env) t} }>.
+Proof.
+  induction env; intros; auto.
+  destruct a. simpl.
+  inversion H0.
+  destruct (s =? x) eqn:Heqb.
+  - apply eqb_eq in Heqb as Heq.
+    subst.
+    rewrite duplicate_subst; auto.
+  - apply eqb_neq in Heqb as Hneq.
+    rewrite swap_subst; eauto.
+Qed.
+
+Lemma subst_msubst' : forall env x v t,
+    closed v ->
+    closed_env env ->
+    msubst_term (drop x env) <{ [v/x]t }> = <{ [v/x] {msubst_term (drop x env) t} }>.
+Proof.
+  induction env; intros; auto.
+  destruct a. simpl.
+  inversion H0.
+  destruct (s =? x) eqn:Heqb.
+  - apply eqb_eq in Heqb as Heq.
+    subst.
+    eauto.
+  - apply eqb_neq in Heqb as Hneq.
+    simpl.  
+    rewrite swap_subst; eauto.
+Qed.
+
+Lemma subst_msubst'' : forall env x xs v t,
+    closed v ->
+    closed_env env ->
+    ~ In x xs ->
+    msubst_term (mdrop xs env) <{ [v/x]t }> = <{ [v/x] {msubst_term (mdrop xs env) t} }>.
+Proof. Admitted.
+
+Lemma subst_bnr__msubst_bnr : forall env x v bs,
+    closed v ->
+    closed_env env ->
+    msubst_bindings_nonrec env <{ [v/x][bnr] bs }> = <{ [v/x][bnr] {msubst_bindings_nonrec (drop x env) bs} }>.
+Proof.
+  induction env; intros; auto.
+  destruct a. simpl.
+  inversion H0.
+  destruct (s =? x) eqn:Heqb.
+  - apply eqb_eq in Heqb as Heq.
+    subst.
+    rewrite duplicate__subst_bnr; auto.
+  - apply eqb_neq in Heqb as Hneq.
+    rewrite swap__subst_bnr; eauto.
+Qed.
+
+Lemma subst_bnr__msubst_bnr' : forall env x v bs,
+    closed v ->
+    closed_env env ->
+    msubst_bindings_nonrec (drop x env) <{ [v/x][bnr] bs }> = <{ [v/x][bnr] {msubst_bindings_nonrec (drop x env) bs} }>.
+Proof. Admitted.
+
+Lemma substA_msubstA : forall envA X U t,
+    Ty.closed U ->
+    msubstA_term envA <{ [[U/X]t }> = <{ [[U/X] {msubstA_term (drop X envA) t} }>.
+Proof. Admitted.
+
+Lemma substA_msubst : forall X U env t,
+    Ty.closed U ->
+    <{ [[U / X] (/[ env /] t ) }> =  <{ /[ env /] ([[U / X] t) }> .
+Proof. Admitted.
+
+(** ** Properties of multi-extensions *)
+
+Lemma mupdate_lookup : forall (c : tass) (x : name),
+    lookup x c = (mupdate empty c) x.
+Proof.
+  induction c.
+  - intros.
+    simpl.
+    reflexivity.
+  - intros.
+    simpl.
+    destruct a.
+    destruct (s =? x) eqn:Heqb.
+    + apply eqb_eq in Heqb as Heq.
+      subst.
+      rewrite update_eq.
+      reflexivity.
+    + apply eqb_neq in Heqb as Hneq.
+      rewrite update_neq; auto.
+Qed.
+
+Lemma mupdate_drop : forall (c : tass) x T,
+    (x |-> T; mupdate empty c) = (x |-> T; mupdate empty (drop x c)).
+Proof. 
+  induction c; intros. 
+  - auto.
+  - destruct a.
+    simpl.
+    destruct (s =? x) eqn:Heqb.
+    + apply eqb_eq in Heqb as Heq.
+      subst.
+      rewrite update_shadow.
+      auto.
+    + apply eqb_neq in Heqb as Hneq.
+      rewrite update_permute; auto.
+      simpl.
+      assert ((x |-> T; s |-> t; mupdate empty (drop x c)) = (s |-> t; x |-> T; mupdate empty (drop x c))). {
+        apply update_permute. auto. 
+      }
+      rewrite H.
+      f_equal.
+      auto.
+Qed.
+
+(*
+Lemma mupdate_drop : forall (c : tass) Gamma x x',
+      lookupT (mupdate Gamma (drop x c)) x' 
+    = if String.eqb x x' 
+        then lookupT Gamma x' 
+        else lookupT (mupdate Gamma c) x'.
+Proof. Admitted.
+*)
+
+Lemma mupdate_unfold : forall {X : Type} (c : list (string * X)) x (v : X),
+    (x |-> v; mupdate empty c) = mupdate empty ((x, v) :: c).
+Proof. intros. auto. Qed.
+
+Lemma mdrop_nil : forall X ns,
+    @mdrop X ns nil = nil.
+Proof. induction ns; auto. Qed.
+
+(** ** Properties of Instantiations *)
+
+(** ** Congruence lemmas on [eval] *)
+
+(** ** Multi-substitutions preserve typing *)
+
+Fixpoint mgsubst (xts : tass) (Gamma : Gamma) : Context.Gamma :=
+  match xts with
+  | nil => Gamma
+  | ((a, T) :: xts') => mgsubst xts' (gsubst a T Gamma)
+  end.
+
+
+
+Lemma mgsubst_nil : forall Gamma,
+    mgsubst nil Gamma = Gamma.
+Proof. intros. apply Coq.Logic.FunctionalExtensionality.functional_extensionality. intros. unfold mgsubst. destruct (Gamma x); auto. Qed.
+
+Lemma mgsubst_absorbs_msubstT : forall xts x T Gamma,
+    mgsubst xts (x |-> T; Gamma) = (x |-> msubstT xts T; mgsubst xts Gamma).
+Proof.
+  induction xts.
+  - auto.
+  - intros.
+    destruct a. 
+    simpl.
+    rewrite <- gsubst_absorbs_substituteT.
+    eauto.
+Qed.
+
+Lemma mgsubst_empty : forall xts,
+    mgsubst xts empty = empty.
+Proof. induction xts; auto. simpl. destruct a. auto. Qed.
+
+Lemma normalise_commutes : forall ss X U T Tn,
+    normalise (msubstT ss (substituteT X U T)) Tn ->
+    exists T0n, 
+      normalise (substituteT X U T) T0n /\
+      normalise (msubstT ss T0n) Tn.
+Proof. Admitted.
+
+Lemma msubstA_preserves_typing_1 : forall rho ck,
+    RD ck rho ->
+    forall Delta Gamma t T Tn,
+      mupdate Delta ck ,, Gamma |-+ t : T ->
+      normalise (msubstT (msyn1 rho) T) Tn ->
+      Delta ,, mgsubst (msyn1 rho) Gamma |-+ (msubstA_term (msyn1 rho) t) : Tn. 
+Proof.
+  intros rho ck V.
+  induction V.
+  - intros.
+    subst.
+    simpl.
+    simpl in H0.
+    apply has_type__normal in H as H1.
+    apply normalisation__stable__normal in H0; auto.
+    subst.
+    assumption.
+  - intros.
+    subst.
+    simpl.
+    simpl in H3.
+    eapply normalise_commutes in H3 as temp.
+    destruct temp as [T0n [Hn1 Hn2]].
+    eapply IHV.
+    + eapply substituteA_preserves_typing.
+      * eauto.
+      * eauto.
+      * apply Hn1.
+    + eassumption. 
+Qed.
+
+Lemma msubstA_preserves_typing_2 : forall rho ck,
+    RD ck rho ->
+    forall Delta Gamma t T Tn,
+      mupdate Delta ck ,, Gamma |-+ t : T ->
+      normalise (msubstT (msyn2 rho) T) Tn ->
+      Delta ,, mgsubst (msyn2 rho) Gamma |-+ (msubstA_term (msyn2 rho) t) : Tn. 
+Proof.
+  intros rho ck V.
+  induction V.
+  - intros.
+    subst.
+    simpl.
+    simpl in H0.
+    apply has_type__normal in H as H1.
+    apply normalisation__stable__normal in H0; auto.
+    subst.
+    assumption.
+  - intros.
+    subst.
+    simpl.
+    simpl in H3.
+    eapply normalise_commutes in H3 as temp.
+    destruct temp as [T0n [Hn1 Hn2]].
+    eapply IHV.
+    + eapply substituteA_preserves_typing.
+      * eauto.
+      * eauto.
+      * apply Hn1.
+    + eassumption. 
+Qed.
+
+Lemma msubst_preserves_typing_1 : forall rho k c e1 e2,
+    RG rho k c e1 e2 ->
+    0 < k ->
+    forall Gamma T t,
+      empty ,, (mgsubst (msyn1 rho) (mupdate Gamma c)) |-+ t : T ->
+      empty ,, (mgsubst (msyn1 rho) Gamma) |-+ (msubst_term e1 t) : T. 
+Proof.
+  intros rho k c e1 e2 V Hlt.
+  induction V.
+  - intros.
+    simpl.
+    assumption.
+  - intros.
+    eapply RV_typable_empty_1 in H as temp; eauto.
+    destruct temp as [Tn'[Hnorm__Tn Htyp__v1]].
+    eapply IHV; eauto.
+    eapply substitution_preserves_typing.
+    + simpl in H1.
+      rewrite mgsubst_absorbs_msubstT in H1.
+      eauto.
+    + eauto.
+    + eauto.
+Qed.
+
+Lemma msubst_preserves_typing_2 : forall rho k c e1 e2,
+    RG rho k c e1 e2 ->
+    0 < k ->
+    forall Gamma T t,
+      empty ,, (mgsubst (msyn2 rho) (mupdate Gamma c)) |-+ t : T ->
+      empty ,, (mgsubst (msyn2 rho) Gamma) |-+ (msubst_term e2 t) : T. 
+Proof.
+  intros rho k c e1 e2 V Hlt.
+  induction V.
+  - intros.
+    simpl.
+    assumption.
+  - intros.
+    eapply RV_typable_empty_2 in H as temp; eauto.
+    destruct temp as [Tn [Hnorm__Tn Htyp__v2]].
+    eapply IHV; eauto.
+    eapply substitution_preserves_typing.
+    + simpl in H1.
+      rewrite mgsubst_absorbs_msubstT in H1.
+      eauto.
+    + eauto.
+    + eauto.
+Qed. 
+
+Lemma msubstT_preserves_kinding_1 : forall ck rho,
+  RD ck rho ->
+  forall Delta T K,
+    (mupdate Delta ck) |-* T : K ->
+    Delta |-* (msubstT (msyn1 rho) T) : K.
+Proof.
+  intros ck rho V.
+  induction V; intros.
+  - assumption.
+  - simpl.
+    eapply IHV.
+    eapply substituteT_preserves_kinding.
+    + apply H2.
+    + assumption.
+Qed.
+
+Lemma msubstT_preserves_kinding_2 : forall ck rho,
+  RD ck rho ->
+  forall Delta T K,
+    (mupdate Delta ck) |-* T : K ->
+    Delta |-* (msubstT (msyn2 rho) T) : K.
+Proof.
+  intros ck rho V.
+  induction V; intros.
+  - assumption.
+  - simpl.
+    eapply IHV.
+    eapply substituteT_preserves_kinding.
+    + apply H2.
+    + assumption.
+Qed.
